Progress, now implementing the ghost queue

share/steel/examples/pulse/parallel/GhostTaskQueue.fsti
@@ -7,7 +7,7 @@ module GR = Pulse.Lib.GhostReference
 open SingleGhostTask
 
 
-let rec is_same_mono_list #a (x y: mono_list a) =
+let rec is_same_mono_list (x y: mono_list) =
 match x, y with
 | [], [] -> True
 | tx::qx, ty::qy ->
@@ -33,7 +33,7 @@ Lemma (is_same_mono_list x y /\ is_same_mono_list y z ==> is_same_mono_list x z)
 | _::qx, _::qy, _::qz -> is_same_trans qx qy qz
 | _ -> ()
 
-let rec is_mono_suffix' #a (x y: mono_list a): prop
+let rec is_mono_suffix' (x y: mono_list): prop
 = if L.length x < L.length y then is_mono_suffix' x (L.tl y)
   else if L.length x = L.length y then is_same_mono_list x y
   else False
@@ -54,30 +54,30 @@ Lemma (requires is_mono_suffix' x y /\ is_mono_suffix' y z)
     else is_same_trans x y z
   )
 
-//val is_mono_suffix (#a: Type): P.preorder (mono_list a)
+//val is_mono_suffix (#a: Type): P.preorder (mono_list)
 
-let is_mono_suffix (#a: Type): P.preorder (mono_list a) =
-  introduce forall x. (is_mono_suffix' #a x x) with (is_mono_suffix_refl #a x);
-  introduce forall x y z. (is_mono_suffix' #a x y /\ is_mono_suffix' y z
+let is_mono_suffix: P.preorder mono_list =
+  introduce forall x. (is_mono_suffix' x x) with (is_mono_suffix_refl x);
+  introduce forall x y z. (is_mono_suffix' x y /\ is_mono_suffix' y z
     ==> is_mono_suffix' x z) with (
-  introduce (is_mono_suffix' #a x y /\ is_mono_suffix' y z)
+  introduce (is_mono_suffix' x y /\ is_mono_suffix' y z)
     ==> is_mono_suffix' x z
     with _. (is_mono_suffix_trans x y z)
   );
   is_mono_suffix'
 
-//val task_in_queue (#a: Type) (x: a) (pos:nat) (l: mono_list a): prop
+//val task_in_queue (#a: Type) (x: a) (pos:nat) (l: mono_list): prop
 
 let task_plus a = a & GR.ref bool & GR.ref bool & GR.ref bool
 
-let rec task_in_queue (#a: Type) (x: task_plus a) (pos:nat) (l: mono_list a): prop =
+let rec task_in_queue (x: task) (pos:nat) (l: mono_list): prop =
   if pos + 1 = L.length l then
     (L.hd l)._1 == x
   else if pos + 1 < L.length l then
     task_in_queue x pos (L.tl l)
   else False
 
-let rec task_in_queue_same_mono #a (t: task_plus a) (pos:nat) (x y: mono_list a):
+let rec task_in_queue_same_mono (t: task) (pos:nat) (x y: mono_list):
 Lemma (requires is_same_mono_list x y)
       (ensures task_in_queue t pos x ==> task_in_queue t pos y)
 = is_same_mono_same_length x y;
@@ -86,8 +86,8 @@ Lemma (requires is_same_mono_list x y)
   else ()
 
 // main reason why we want this preorder:
-let rec task_in_queue_preorder #a 
-    (t: task_plus a) (pos: nat) (x y: mono_list a):
+let rec task_in_queue_preorder
+    (t: task) (pos: nat) (x y: mono_list):
 Lemma (requires task_in_queue t pos x /\ is_mono_suffix x y)
       (ensures task_in_queue t pos y)
 = if L.length x < L.length y then task_in_queue_preorder t pos x (L.tl y)
@@ -95,30 +95,30 @@ Lemma (requires task_in_queue t pos x /\ is_mono_suffix x y)
 
 // 1. enqueue: when spawning a new task
 // get a certificate for task_in_queue
-let enqueue_todo #a (l: mono_list a) (t: task_plus a)
+let enqueue_todo (l: mono_list) (t: task)
 (*
-(r:mono_list a{ get_actual_queue r == t::get_actual_queue l
+(r:mono_list{ get_actual_queue r == t::get_actual_queue l
                 /\ count_ongoing r == count_ongoing l } &
 pos:nat{task_in_queue t pos r})
 *)
 = (| (t, Todo)::l, L.length l |)
 
-let enqueue_preserves_order #a l (t: task_plus a):
+let enqueue_preserves_order l (t: task):
 Lemma (is_mono_suffix l (enqueue_todo l t)._1)
 = is_same_refl l
 
-let rec count_ongoing #a (l: mono_list a): nat =
+let rec count_ongoing (l: mono_list): nat =
 match l with
 | [] -> 0
 | t::q -> (if t._2 = Ongoing then 1 else 0) + count_ongoing q
 
-let get_actual_queue #a (l: mono_list a): list a =
-    L.map (fun (t: extended_task a) -> t._1._1) (L.filter is_Todo l)
+let get_actual_queue (l: mono_list): list task =
+    L.map (fun (t: extended_task) -> t._1) (L.filter is_Todo l)
 
 // 2. pop: when a worker starts working on a task
 // it updates the task to "ongoing"
-let rec pop_todo_task #a (l: mono_list a{~(get_actual_queue l == [])})
-: (t:task_plus a & r:mono_list a{ get_actual_queue l == t._1::get_actual_queue r
+let rec pop_todo_task (l: mono_list{~(get_actual_queue l == [])})
+: (t:task & r:mono_list{ get_actual_queue l == t::get_actual_queue r
                 /\ count_ongoing r == count_ongoing l + 1 }
   & pos:nat{task_in_queue t pos r})
 = match l with
@@ -147,11 +147,11 @@ let task_in_queue_not_empty t pos l:
         (ensures L.length l >= 1)
 = ()
 
-let rec close_task #a
-    (t: task_plus a)
+let rec close_task
+    (t: task)
     (pos: nat)
-    (l: mono_list a{task_in_queue t pos l /\ L.length l >= 1}):
-    (s:task_status{L.memP (t, s) l} & r:mono_list a{
+    (l: mono_list{task_in_queue t pos l /\ L.length l >= 1}):
+    (s:task_status{L.memP (t, s) l} & r:mono_list{
         s == Ongoing ==> (
             get_actual_queue r == get_actual_queue l /\
             count_ongoing r == count_ongoing l - 1)})
@@ -160,21 +160,23 @@ if pos + 1 = L.length l
   then (| s, (t', Done)::q |) // if s is not Ongoing, then we have too much permission
   else let (| s', q' |) = close_task t pos q in (| s', (t', s)::q' |)
 
-let rec close_task_preserves_order_aux #a
-    (t: task_plus a)
+let rec close_task_preserves_order_aux
+    (t: task)
     (pos: nat)
-    (l: mono_list a{task_in_queue t pos l}):
+    (l: mono_list{task_in_queue t pos l}):
     Lemma (is_same_mono_list l (close_task t pos l)._2 )
 = match l with
 | (t', s)::q -> if pos + 1 = L.length l then is_mono_suffix_refl q
 else let (| s', q' |) = close_task t pos q in close_task_preserves_order_aux t pos q
 
-let close_task_preserves_order #a
-    (t: task_plus a)
+let close_task_preserves_order
+    (t: task)
     (pos: nat)
-    (l: mono_list a{task_in_queue t pos l}):
+    (l: mono_list{task_in_queue t pos l}):
     Lemma (is_mono_suffix l (close_task t pos l)._2 )
 = close_task_preserves_order_aux t pos l; from_same_to_suffix l (close_task t pos l)._2
+
+
 
 
 (** ------------------------------------------------------
@@ -187,25 +189,25 @@ open Pulse.Lib.Pervasives
 #push-options "--print_universes"
 
 //unfold
-let ghost_mono_ref a = M.ref (mono_list a) is_mono_suffix
+let ghost_mono_ref = M.ref mono_list is_mono_suffix
 
 (*
-let pts_to_ghost_queue #a (r: ghost_mono_ref a) (l: mono_list a): vprop
+let pts_to_ghost_queue #a (r: ghost_mono_ref) (l: mono_list): vprop
 = M.pts_to r full_perm l
 
 //open Pulse.Lib.Pervasives
 
-let pts_to_ghost_queue_half #a (r: ghost_mono_ref a) (l: mono_list a): vprop
+let pts_to_ghost_queue_half #a (r: ghost_mono_ref) (l: mono_list): vprop
 = M.pts_to r one_half l
 *)
 
 (* Share/gather specialized to half permission *)
-val mono_share2 (#a:Type) (r:ghost_mono_ref a) (#v:erased (mono_list a))
+val mono_share2 (#a:Type) (r:ghost_mono_ref) (#v:erased (mono_list))
   : stt_ghost unit
       (M.pts_to r full_perm v)
       (fun _ -> M.pts_to r one_half v ** M.pts_to r one_half v)
 
-val mono_gather2 (#a:Type) (r:ghost_mono_ref a) (#x0 #x1: erased (mono_list a))
+val mono_gather2 (#a:Type) (r:ghost_mono_ref) (#x0 #x1: erased (mono_list))
   : stt_ghost unit
       (M.pts_to r one_half x0 ** M.pts_to r one_half x1)
       (fun _ -> M.pts_to r full_perm x0 ** pure (x0 == x1))
@@ -218,9 +220,9 @@ Lemma (P.stable (task_in_queue t pos) is_mono_suffix)
   ==> task_in_queue t pos y with _. task_in_queue_preorder t pos x y)
 
 // can witness that task is in queue
-let witness (#a:Type) #t #pos
-            (r:ghost_mono_ref a)
-            (v:erased (mono_list a))
+let witness #t #pos
+            (r:ghost_mono_ref)
+            (v:erased (mono_list))
             (_:squash (task_in_queue t pos v))
   : //TODO: SteelAtomicUT
   stt_ghost (M.witnessed r (task_in_queue t pos)) 
@@ -228,9 +230,9 @@ let witness (#a:Type) #t #pos
                   (fun _ -> M.pts_to r full_perm v)
 = task_in_queue_stable t pos ; M.witness r (task_in_queue t pos) v _
 
-let recall (#a:Type u#1) #t #pos
-           (r:ghost_mono_ref a)
-           (v:erased (mono_list a))
+let recall #t #pos
+           (r:ghost_mono_ref)
+           (v:erased (mono_list))
            (w:M.witnessed r (task_in_queue t pos))
   : //TODO: SteelAtomicU
  stt_ghost unit 
@@ -238,9 +240,9 @@ let recall (#a:Type u#1) #t #pos
                  (fun _ -> M.pts_to r one_half v ** pure (task_in_queue t pos v))
   = M.recall (task_in_queue t pos) r v w
 
-let recall_full (#a:Type u#1) #t #pos
-           (r:ghost_mono_ref a)
-           (v:erased (mono_list a))
+let recall_full #t #pos
+           (r:ghost_mono_ref)
+           (v:erased (mono_list))
            (w:M.witnessed r (task_in_queue t pos))
   : //TODO: SteelAtomicU
  stt_ghost unit 
@@ -255,7 +257,8 @@ let recall_full (#a:Type u#1) #t #pos
 
 module Lock = Pulse.Lib.SpinLock
 
-let task_elem: Type u#1 = (
+(*
+let task: Type u#1 = (
   a: Type0 // return type of the computation
   & r: ref (option a) // the reference where we put the result of the computation
   & Lock.lock (own_res r)//(exists_ (fun v -> pts_to r half v ** (if None? v then pts_to r half v else emp)))
@@ -263,124 +266,130 @@ let task_elem: Type u#1 = (
   // to create this thing
 )
 
+let task_plus: Type u#1 = task_with_status task
 
+let mono_list_task_plus: Type u#1 = mono_list task
+*)
 
-let task_plus: Type u#1 = task_with_status task_elem
-
-let mono_list_task_plus: Type u#1 = mono_list task_elem
-
-let certificate (r:ghost_mono_ref task_elem) (t: task_elem) (pos: nat)
+let certificate (r:ghost_mono_ref) (t: task) (pos: nat)
 = M.witnessed r (task_in_queue t pos)
 
 // can witness that task is in queue
-let get_certificate (t: task_elem) (pos: nat)
-            (r:ghost_mono_ref task_elem)
-            (l:mono_list_task_plus)
+let get_certificate (t: task) (pos: nat)
+            (r:ghost_mono_ref)
+            (l:mono_list)
             (_:squash (task_in_queue t pos l))
   : //TODO: SteelAtomicUT
   stt_ghost (certificate r t pos)
-            emp_inames
                   (M.pts_to r full_perm l)
                   (fun _ -> M.pts_to r full_perm l)
 = witness r l _
 
-let pts_to_Some (t: task_elem & task_status) (f: perm): vprop
-= (exists_ (fun v -> pts_to (t._1._2) #f v ** pure (Some? v)))
-
-//let pts_to_Some (t: task_elem & task_status): vprop
-//= (exists_ (fun v -> pts_to (t._1._2) #three_quart v ** pure (Some? v)))
 
 
 
-let task_res_own (t: task_plus) (f: perm): vprop
-= match t._2 with
-| Todo -> pts_to (t._1._2) #f None // three_quarter
-| Ongoing -> emp // in this case, the worker has the half permission
-| Done -> pts_to_Some t f  //(exists_ (fun v -> pts_to (t._1._2) #three_quart v ** pure (Some? v)))
-
-(*
-let task_res_own (t: task_plus): vprop
-= match t._2 with
-| Todo -> pts_to (t._1._2) #three_quart None
-| Ongoing -> emp // in this case, the worker has the half permission
-| Done -> pts_to_Some t //(exists_ (fun v -> pts_to (t._1._2) #three_quart v ** pure (Some? v)))
-*)
 
 
 
-let rec tasks_res_own (l: mono_list_task_plus) (f: perm): vprop
-=  match l with
-  | [] -> emp
-  | tl::ql -> task_res_own tl f ** tasks_res_own ql f
-  
-(*
-let rec tasks_res_own (l: mono_list_task_plus): vprop
-=  match l with
-  | [] -> emp
-  | tl::ql -> task_res_own tl ** tasks_res_own ql
-*)
+
+
+#pop-options
+
+let inv_ghost_queue (r: ghost_mono_ref): vprop =
+  exists* l. M.pts_to r one_half l ** tasks_res l
 
 ```pulse
 ghost
-fn fold_done_task (t: task_elem) (l:mono_list_task_plus) (f: perm)
-  requires pts_to t._2 #f None ** tasks_res_own l f
-  ensures tasks_res_own (enqueue_todo l t)._1 f
+fn add_todo_task (t: task) (l:mono_list)
+  requires GR.pts_to t._1 #one_half true ** GR.pts_to t._2 #one_half false ** pts_to t._4 #one_half false ** GR.pts_to t._5 #one_half false
+   ** tasks_res l
+  ensures tasks_res (enqueue_todo l t)._1
 {
-  rewrite (pts_to t._2 #f None) as (task_res_own (t, Todo) f);
-  fold (task_res_own (t, Todo) f);
-  rewrite (task_res_own (t, Todo) f ** tasks_res_own l f)
-    as
-  (tasks_res_own (enqueue_todo l t)._1 f);
+  get_task_res_todo t;
+  assert (task_res (t, Todo) ** tasks_res l);
+  rewrite (task_res (t, Todo) ** tasks_res l) as tasks_res (enqueue_todo l t)._1;
   ()
 }
 ```
 
 (*
-Old version:
-let small_inv (r: ghost_mono_ref task_elem) (q: list task_elem) (c: int): vprop 
-= exists_ (fun l -> M.pts_to r full_perm l **
-  tasks_res_own l **
-  pure (count_ongoing l = c /\ get_actual_queue l == q)
-)
+Needed:
+1. Create ghost queue empty, invariant (with half permission)
+We give back the other half
 *)
 
-//let three_eight = half_perm three_quart
+(* TD: Current progress here... *)
 
-// TODO: Implement as a case distinction
+(*
+// 1. create queue, alloc inv
 ```pulse
-ghost fn
-share_task_res_own_generic t (f1 f2: perm)
-requires task_res_own t (sum_perm f1 f2)
-ensures task_res_own t f1 ** task_res_own t f2
+unobservable fn init_ghost_queue' (_: unit)
+requires emp
+returns res: (r:ghost_mono_ref & inv (inv_ghost_queue r))
+ensures M.pts_to res._1 one_half []
 {
+  let r = M.alloc #_ #is_mono_suffix [];
+
   admit()
+  (*
+  let l: mono_list task = [(t, Todo)];
+  let r': M.ref (mono_list task) is_mono_suffix = M.alloc #emp_inames #_ (is_mono_suffix) l;
+  assert (M.pts_to r' full_perm l);
+  let r: gmref = convert_to_ghost_mono_ref r';
+
+  rewrite (M.pts_to r' full_perm l) as (M.pts_to r full_perm l);
+  let w: certificate r t 0 = get_certificate t 0 r l _;
+
+
+  let pair': (r:gmref & certificate r t 0) = (| r, w |);
+  let pair: erased (r:gmref & certificate r t 0) = hide pair';
+
+  share_queue r l;
+  assert (pure (count_ongoing l = 0 /\ get_actual_queue l == [t]));
+  // now: create tasks_res_own
+  //share pts_to t._2 #three_quart None
+  //share pts_to t._2
+  fold (task_res_own (t, Todo) three_quart);
+  rewrite emp as (tasks_res_own [] three_quart);
+  rewrite (task_res_own (t, Todo) three_quart ** tasks_res_own [] three_quart) as
+    (tasks_res_own l three_quart);
+  //fold (task_res_own t one_quart);
+  share_tasks_res_own l;
+  rewrite (M.pts_to r one_half l ** tasks_res_own l one_quart)
+    as `@(if 1 = 0 && L.length [t] = 0 then deadline r
+  else M.pts_to r one_half l ** tasks_res_own l one_quart);
+  fold small_inv r [t] 0;
+  rewrite (small_inv r [t] 0) as (small_inv (reveal pair)._1 [t] 0);
+  pair
+  *)
 }
 ```
 
-```pulse
-ghost fn
-gather_task_res_own_generic t (f1 f2: perm)
-requires task_res_own t f1 ** task_res_own t f2
-ensures task_res_own t (sum_perm f1 f2)
-{
-  admit()
-}
-```
+let init_ghost_queue = init_ghost_queue'
 
 
 
-```pulse
-ghost fn
-share_task_res_own t (f: perm)
-requires task_res_own t f
-ensures task_res_own t (half_perm f) ** task_res_own t (half_perm f)
-{
-  rewrite task_res_own t f
-    as (task_res_own t (sum_perm (half_perm f) (half_perm f)));
-  share_task_res_own_generic t (half_perm f) (half_perm f);
-  ()
-}
-```
+
+
+
+
+
+
+
+
+
+
+
+
+
+
+
+
+
+
+
+
+(*
 
 // assuming because of universe polymorphism
 assume val
@@ -389,326 +398,21 @@ stt_return #a (x:a): stt a emp (fun y -> pure (x == y))
 // assuming because of universe polymorphism
 assume val
 stt_return_ghost #a (x:a): stt_ghost a emp_inames emp (fun y -> pure (x == y))
+*)
 
-// Assuming recursion
-assume val share_tasks_res_own_generic_cb (p: mono_list_task_plus) (f1: perm) (f2: perm):
-stt_ghost unit emp_inames (tasks_res_own p (sum_perm f1 f2))
-(fun () -> tasks_res_own p f1 ** tasks_res_own p f2)
-
-```pulse
-ghost fn
-share_tasks_res_own_generic (l: mono_list_task_plus) (f1: perm) (f2: perm)
-requires tasks_res_own l (sum_perm f1 f2)
-ensures tasks_res_own l f1 ** tasks_res_own l f2
-{
-  if (L.length l = 0)
-  {
-    rewrite (tasks_res_own l (sum_perm f1 f2)) as emp;
-    rewrite emp as (tasks_res_own l f1);
-    rewrite emp as (tasks_res_own l f2);
-    ()
-  }
-  else {
-    let tl = stt_return_ghost (L.hd l);
-    let ql = stt_return_ghost (L.tl l);
-    rewrite (tasks_res_own l (sum_perm f1 f2))
-      as (task_res_own tl (sum_perm f1 f2) ** tasks_res_own ql (sum_perm f1 f2));
-    share_task_res_own_generic tl f1 f2;
-    share_tasks_res_own_generic_cb ql f1 f2;
-    rewrite (task_res_own tl f1 ** tasks_res_own ql f1)
-      as (tasks_res_own l f1);
-    rewrite (task_res_own tl f2 ** tasks_res_own ql f2)
-      as (tasks_res_own l f2);
-    ()
-  }
-}
-```
-
-```pulse
-ghost fn
-share_tasks_res_own_general (p: mono_list_task_plus) (f: perm)
-requires tasks_res_own p f
-ensures tasks_res_own p (half_perm f) ** tasks_res_own p (half_perm f)
-{
-  rewrite (tasks_res_own p f) as (tasks_res_own p (sum_perm (half_perm f) (half_perm f)));
-  share_tasks_res_own_generic p (half_perm f) (half_perm f);
-  ()
-}
-```
-
-// assuming recursion
-assume val gather_tasks_res_own_cb (l: mono_list_task_plus) (f1 f2: perm)
-: stt_ghost unit emp_inames (tasks_res_own l f1 ** tasks_res_own l f2)
-(fun () -> tasks_res_own l (sum_perm f1 f2))
-
-```pulse
-ghost fn gather_tasks_res_own (l: mono_list_task_plus) (f1 f2: perm)
-requires tasks_res_own l f1 ** tasks_res_own l f2
-ensures tasks_res_own l (sum_perm f1 f2)
-{
-  if (L.length l = 0) {
-    rewrite (tasks_res_own l f1) as emp;
-    rewrite (tasks_res_own l f2) as emp;
-    rewrite emp as (tasks_res_own l (sum_perm f1 f2));
-    ()
-  }
-  else
-  {
-    let tl = stt_return_ghost (L.hd l);
-    let ql = stt_return_ghost (L.tl l);
-    rewrite (tasks_res_own l f1) as (task_res_own tl f1 ** tasks_res_own ql f1);
-    rewrite (tasks_res_own l f2) as (task_res_own tl f2 ** tasks_res_own ql f2);
-    gather_task_res_own_generic tl f1 f2;
-    gather_tasks_res_own_cb ql f1 f2;
-    rewrite (task_res_own tl (sum_perm f1 f2) ** tasks_res_own ql (sum_perm f1 f2))
-      as (tasks_res_own l (sum_perm f1 f2));
-    ()
-  }
-}
-```
-
-
-
-```pulse
-ghost fn
-share_tasks_res_own (p: mono_list_task_plus)
-requires tasks_res_own p three_quart
-ensures tasks_res_own p one_half ** tasks_res_own p one_quart
-{
-  rewrite (tasks_res_own p three_quart)
-    as (tasks_res_own p (sum_perm one_half one_quart));
-  share_tasks_res_own_generic p one_half one_quart;
-  ()
-}
-```
-
-
-
-
-
-let deadline (r: ghost_mono_ref task_elem): vprop
-= exists_ (fun f1 ->
-  exists_ (fun f2 ->
-  exists_ (fun l ->
-    M.pts_to r f1 l ** tasks_res_own l f2
-    ** pure (count_ongoing l = 0 /\ get_actual_queue l == [])
-  )))
-
-```pulse
-ghost fn
-duplicate_deadline' (r: ghost_mono_ref task_elem)
-requires deadline r
-ensures deadline r ** deadline r
-{
-  unfold deadline r;
-  with f1 f2 l. assert (M.pts_to r f1 l ** tasks_res_own l f2
-    ** pure (count_ongoing l = 0 /\ get_actual_queue l == []));
-  M.share #emp_inames r f1 l;
-  share_tasks_res_own_general l f2;
-  fold deadline r;
-  fold deadline r;
-  ()
-}
-```
-
-let duplicate_deadline = duplicate_deadline'
-
-```pulse
-ghost fn
-obtain_deadline (r: ghost_mono_ref task_elem) (f: perm)
-requires (exists l. M.pts_to r one_half l ** tasks_res_own l f **
-      pure (count_ongoing l = 0 /\ get_actual_queue l == []))
-  ensures deadline r
-{
-  with l. assert (M.pts_to r one_half l **
-      pure (count_ongoing l = 0 /\ get_actual_queue l == []));
-  unfold M.pts_to r one_half l;
-  assert (M.pts_to r one_half l ** pure (count_ongoing l = 0 /\ get_actual_queue l == []));
-  fold deadline r;
-  ()
-}
-```
-
-let small_inv (r: erased (ghost_mono_ref task_elem)) (q: list task_elem) (c: int): vprop 
-= exists_ (fun l -> M.pts_to r one_half l **
-  tasks_res_own l one_half **
-  pure (count_ongoing l = c /\ get_actual_queue l == q)
-  ** (if c = 0 && L.length q = 0 then deadline r
-  else M.pts_to r one_half l ** tasks_res_own l one_quart)
-)
-
-```pulse
-ghost fn
-extract_deadline' (r: gmref)
-requires small_inv r [] 0
-ensures small_inv r [] 0 ** deadline r
-{
-  unfold small_inv r [] 0;
-  with l. assert (pts_to_ghost_queue_half (reveal r) l);
-  // FIXME: why do we need reveal r here?
-  rewrite `@(if (0<:nat) = 0 && L.length ([] <: list task_elem) = 0 then deadline r
-    else M.pts_to r one_half l ** tasks_res_own l one_quart)
-  as deadline r;
-  duplicate_deadline r;
-  rewrite deadline r 
-    as `@(if (0<:nat) = 0 && L.length ([] <: list task_elem) = 0 then deadline r
-    else M.pts_to r one_half l ** tasks_res_own l one_quart);
-  fold small_inv r [] 0;
-  ()
-}
-```
-
-let extract_deadline = extract_deadline'
-
-```pulse
-ghost
-fn unfold_small_inv
-(r: gmref) (q: list task_elem) (c: int)
-requires small_inv r q c ** pure (c > 0 \/ L.length q > 0)
-ensures exists l. (M.pts_to r full_perm l
-  ** tasks_res_own l three_quart
-  ** pure (c = count_ongoing l /\ q == get_actual_queue l) 
-)
-{
-  unfold small_inv r q c;
-  with l. assert (pts_to_ghost_queue_half (reveal r) l);
-  rewrite `@(if c = 0 && L.length q = 0 then deadline r
-  else M.pts_to r one_half l ** tasks_res_own l one_quart)
-    as (M.pts_to r one_half l ** tasks_res_own l one_quart);
-  //share_queue_general r l ;
-  rewrite (pts_to_ghost_queue_half (reveal (hide r)) (reveal l))
-    as (M.pts_to r one_half (reveal l));
-  // FIXME: This rewrite should not be needed
-  gather_queue r l l;
-  gather_tasks_res_own l one_half one_quart;
-  rewrite (tasks_res_own l (sum_perm one_half one_quart))
-    as (tasks_res_own l three_quart);
-  ()
-}
-```
-
-```pulse
-ghost
-fn fold_small_inv
-(r: gmref) (q: list task_elem) (c: int)
-requires exists l. (M.pts_to r full_perm l
-  ** tasks_res_own l three_quart
-  ** pure (c = count_ongoing l /\ q == get_actual_queue l)
-  ** pure (c > 0 \/ L.length q > 0)
-  )
-ensures small_inv r q c
-{
-  with l. assert (M.pts_to r full_perm l
-  ** tasks_res_own l three_quart
-  ** pure (c = count_ongoing l /\ q == get_actual_queue l)
-  ** pure (c > 0 \/ L.length q > 0)
-  );
-  share_queue r l;
-  rewrite (tasks_res_own l three_quart)
-    as (tasks_res_own l (sum_perm one_half one_quart));
-  share_tasks_res_own_generic l one_half one_quart;
-  rewrite (M.pts_to r one_half l ** tasks_res_own l one_quart)
-  as `@(if c = 0 && L.length q = 0 then deadline r
-  else M.pts_to r one_half l ** tasks_res_own l one_quart);
-  fold small_inv r q c;
-  ()
-}
-```
 
 
 #push-options "--print_universes --print_implicits"
 
-assume val pts_to_perm (#a: _) (#p: _) (#v: _) (r: ref a)
-  : stt_ghost unit emp_inames
-      (pts_to r #p v)
-      (fun _ -> pts_to r #p v ** pure (p `lesser_equal_perm` full_perm))
     
-let hperm = (f:perm{lesser_equal_perm one_half f})
-
-```pulse
-ghost
-fn derive_false_from_too_much_permission
-(#a: Type) (r: ref a) (v1 v2: a) (f: hperm)
-requires pts_to r #f v1 ** pts_to r #three_quart v2
-ensures pts_to r #f v1 ** pts_to r #three_quart v2
-  ** pure (~(r == r))
-{
-  gather #_ #emp_inames r #v1 #v2 #f #three_quart;
-  pts_to_perm #_ #(sum_perm f three_quart) #v1 r;
-  assert (pure False);
-  share #_ #emp_inames r #v1 #(sum_perm f three_quart);
-  rewrite (pts_to r #(half_perm (sum_perm f three_quart)) v1 **
-    pts_to r #(half_perm (sum_perm f three_quart)) v1)
-  as (pts_to r #f v1 ** pts_to r #three_quart v2);
-  ()
-}
-```
-
-```pulse
-ghost
-fn derive_status_ongoing (h: (task_elem & task_status)) (x: option h._1._1) (f: hperm)
-  requires task_res_own h f ** (pts_to (h._1._2) #three_quart x)
-  ensures task_res_own h f ** (pts_to (h._1._2) #three_quart x) ** pure (h._2 = Ongoing)
-{
-  if (snd h = Todo) {
-    rewrite (task_res_own h f) as (pts_to (h._1._2) #f None);
-    derive_false_from_too_much_permission h._1._2 None x f;
-    assert (pure (h._2 = Ongoing));
-    rewrite (pts_to (h._1._2) #f None) as (task_res_own h f);
-    ()
-  }
-  else {
-    if (snd h = Done) {
-      rewrite (task_res_own h f) as (pts_to_Some h f);
-      unfold (pts_to_Some h f);
-      assert (exists_ (fun v -> pts_to (h._1._2) #f v ** pure (Some? v)));
-      with v. assert (pts_to (h._1._2) #f v ** pure (Some? v));
-      derive_false_from_too_much_permission h._1._2 v x f;
-      fold (pts_to_Some h f);
-      rewrite (pts_to_Some h f) as (task_res_own h f);
-      ()
-    }
-    else {
-      ()
-    }
-  }
-}
-```
 
 
 
-// waiting to have recursion in Pulse
-assume val prove_task_ongoing_aux_cb
-  (t: task_elem)
-  (pos: nat)
-  (v: option t._1)
-  (l: (l:mono_list_task_plus{task_in_queue t pos l /\ L.length l >= 1}))
-  (f: hperm)
-:
-stt_ghost unit emp_inames
-(tasks_res_own l f ** pts_to t._2 #three_quart v)
-(fun () -> tasks_res_own l f  ** pts_to t._2 #three_quart v
-  ** pure (count_ongoing l > 0))
-
-```pulse
-ghost
-fn fold_tasks_res_own
-  (h: (task_elem & task_status)) (q: mono_list_task_plus)
-  (f: hperm)
-requires task_res_own h f ** tasks_res_own q f
-ensures tasks_res_own (h::q) f
-{
-  rewrite (task_res_own h f ** tasks_res_own q f) as (tasks_res_own (h::q) f);
-  ()
-}
-```
-
-
-
+(*
 ```pulse
 ghost
 fn prove_task_ongoing_aux
-  (t: task_elem)
+  (t: task)
   (pos: nat)
   (v: option t._1)
   (l: (l:mono_list_task_plus{task_in_queue t pos l /\ L.length l >= 1}))
@@ -755,12 +459,12 @@ ensures tasks_res_own l f ** pts_to t._2 #three_quart v ** pure (count_ongoing l
 ```pulse
 ghost
 fn prove_task_ongoing'
-  (#t: task_elem)
+  (#t: task)
   (#pos: nat)
   (#v: option t._1)
   (r: gmref)
-  (q: list task_elem) (c: int)
-  //(l: (l:mono_list task_elem{task_in_queue t pos l /\ L.length l >= 1})):
+  (q: list task) (c: int)
+  //(l: (l:mono_list task{task_in_queue t pos l /\ L.length l >= 1})):
   (w:certificate r t pos)
 //stt_ghost unit emp_inames
 requires small_inv r q c ** pts_to t._2 #three_quart v
@@ -768,7 +472,7 @@ ensures small_inv r q c ** pts_to t._2 #three_quart v ** pure (c > 0)
 {
   unfold small_inv r q c;
   with l. assert (M.pts_to r one_half l);
-  let proof = recall #task_elem #t #pos r l w;
+  let proof = recall #task #t #pos r l w;
   assert (pure (task_in_queue t pos l));
   assert (pure (L.length l >= 1));
   prove_task_ongoing_aux t pos v l one_half;
@@ -789,51 +493,13 @@ ensures small_inv r q c ** pts_to t._2 #three_quart v ** pure (c > 0)
 
 *)
 
-let convert_to_ghost_mono_ref (r: M.ref (mono_list task_elem) is_mono_suffix):
+let convert_to_ghost_mono_ref (r: M.ref (mono_list task) is_mono_suffix):
   gmref
-  //ghost_mono_ref task_elem
+  //ghost_mono_ref
   = r
 
-// 0. init queue with task
-```pulse
-ghost fn init_ghost_queue' (t: task_elem)
-requires pts_to t._2 #three_quart None
-returns pair: erased (r: gmref & certificate r t 0)
-ensures small_inv (reveal pair)._1 [t] 0
-{
-  let l: mono_list task_elem = [(t, Todo)];
-  let r': M.ref (mono_list task_elem) is_mono_suffix = M.alloc #emp_inames #_ (is_mono_suffix) l;
-  assert (M.pts_to r' full_perm l);
-  let r: gmref = convert_to_ghost_mono_ref r';
+  *)
 
-  rewrite (M.pts_to r' full_perm l) as (M.pts_to r full_perm l);
-  let w: certificate r t 0 = get_certificate t 0 r l _;
-
-
-  let pair': (r:gmref & certificate r t 0) = (| r, w |);
-  let pair: erased (r:gmref & certificate r t 0) = hide pair';
-
-  share_queue r l;
-  assert (pure (count_ongoing l = 0 /\ get_actual_queue l == [t]));
-  // now: create tasks_res_own
-  //share pts_to t._2 #three_quart None
-  //share pts_to t._2
-  fold (task_res_own (t, Todo) three_quart);
-  rewrite emp as (tasks_res_own [] three_quart);
-  rewrite (task_res_own (t, Todo) three_quart ** tasks_res_own [] three_quart) as
-    (tasks_res_own l three_quart);
-  //fold (task_res_own t one_quart);
-  share_tasks_res_own l;
-  rewrite (M.pts_to r one_half l ** tasks_res_own l one_quart)
-    as `@(if 1 = 0 && L.length [t] = 0 then deadline r
-  else M.pts_to r one_half l ** tasks_res_own l one_quart);
-  fold small_inv r [t] 0;
-  rewrite (small_inv r [t] 0) as (small_inv (reveal pair)._1 [t] 0);
-  pair
-}
-```
-
-let init_ghost_queue = init_ghost_queue'
 
 
 
@@ -842,7 +508,7 @@ let init_ghost_queue = init_ghost_queue'
 ghost
 fn spawn_task_ghost'
 (r: gmref)
-(q: list task_elem) (c: int) (t: task_elem)
+(q: list task) (c: int) (t: task)
 (ct: current_task r)
   requires small_inv r q c ** pts_to t._2 #three_quart None ** is_active ct
   returns w: erased (pos:nat & certificate r t pos)
@@ -859,10 +525,10 @@ fn spawn_task_ghost'
   with vl. assert (M.pts_to r full_perm vl);
   assert (tasks_res_own vl three_quart);
   assert (pure (count_ongoing vl = c /\ get_actual_queue vl == q));
-  let p = enqueue_todo #task_elem vl t;
+  let p = enqueue_todo #task vl t;
   let pos = p._2;
   assert (pure (task_in_queue t pos p._1));
-  write_ghost_queue #task_elem #vl r p._1;
+  write_ghost_queue #task #vl r p._1;
   assert (M.pts_to r full_perm p._1);
   let w: certificate r t pos = get_certificate t pos r p._1 _;
   assert (tasks_res_own vl three_quart);
@@ -930,8 +596,8 @@ let mk_erased_pair #r #t (pos: nat) (w: certificate r t pos):
 ghost
 fn pop_task_ghost'
 (r: gmref)
-(t: task_elem)
-(q: list task_elem) (c: int)
+(t: task)
+(q: list task) (c: int)
 //(ct: current_task r)
   requires small_inv r (t::q) c //** is_active ct
   returns pair:erased (pos:nat & certificate r t pos)
@@ -948,9 +614,9 @@ fn pop_task_ghost'
   with l. assert (M.pts_to r full_perm l);
   assert (tasks_res_own l three_quart);
   assert (pure (count_ongoing l = c /\ get_actual_queue l == t::q));
-  let p = pop_todo_task #task_elem l;
-  let order_is_preserved = pop_preserves_order #task_elem l;
-  write_ghost_queue #task_elem #l r p._2;
+  let p = pop_todo_task #task l;
+  let order_is_preserved = pop_preserves_order #task l;
+  write_ghost_queue #task #l r p._2;
   assert (M.pts_to r full_perm p._2);
   let certif: certificate r t p._3 = get_certificate t p._3 r p._2 ();
   assert (M.pts_to r full_perm p._2);
@@ -979,8 +645,8 @@ let pop_task_ghost = pop_task_ghost'
 let rec close_task_bis #a
     (t: a)
     (pos: nat)
-    (l: mono_list a{task_in_queue t pos l /\ L.length l >= 1}):
-  mono_list a
+    (l: mono_list{task_in_queue t pos l /\ L.length l >= 1}):
+  mono_list
 = let (t', s)::q = l in
 if pos + 1 = L.length l
   then (t', Done)::q // if s is not Ongoing, then we have too much permission
@@ -989,7 +655,7 @@ if pos + 1 = L.length l
 let rec close_task_bis_preserves_order_aux #a
     (t: a)
     (pos: nat)
-    (l: mono_list a{task_in_queue t pos l}):
+    (l: mono_list{task_in_queue t pos l}):
     Lemma (is_same_mono_list l (close_task_bis t pos l) )
 = match l with
 | (t', s)::q -> if pos + 1 = L.length l then is_mono_suffix_refl q
@@ -1000,14 +666,14 @@ else let q' = close_task_bis t pos q in close_task_bis_preserves_order_aux t pos
 let close_task_bis_preserves_order #a
     (t: a)
     (pos: nat)
-    (l: mono_list a{task_in_queue t pos l}):
+    (l: mono_list{task_in_queue t pos l}):
     Lemma (is_mono_suffix l (close_task_bis t pos l) )
 = close_task_bis_preserves_order_aux t pos l; from_same_to_suffix l (close_task_bis t pos l)
 
 
 ```pulse
 ghost
-fn fold_task_done (h:(task_elem & task_status)) (f: perm)
+fn fold_task_done (h:(task & task_status)) (f: perm)
   requires pts_to h._1._2 #f (Some x) ** pure (h._2 = Done)
   ensures task_res_own h f
 {
@@ -1021,7 +687,7 @@ fn fold_task_done (h:(task_elem & task_status)) (f: perm)
 
 // waiting to have recursion in Pulse
 assume val put_back_permission_cb
-  (t: task_elem)
+  (t: task)
   (pos: nat)
   (l: (l:mono_list_task_plus{task_in_queue t pos l /\ L.length l >= 1}))
   (x: t._1)
@@ -1035,10 +701,10 @@ stt_ghost unit emp_inames
 ```pulse
 ghost
 fn fold_tasks_res_own_bis
-  (h: (task_elem & task_status)) 
-  (h': (task_elem & task_status))
+  (h: (task & task_status)) 
+  (h': (task & task_status))
   (q: mono_list_task_plus)
- (pos: nat) (t: task_elem)
+ (pos: nat) (t: task)
 (l: (l:mono_list_task_plus{task_in_queue t pos l /\ b2t (L.length l >= 1)}))
 requires task_res_own h' three_quart ** tasks_res_own q three_quart
   ** pure (t == h._1 /\ h == L.hd l /\ q == L.tl l /\ h' == (h._1, Done)
@@ -1046,11 +712,11 @@ requires task_res_own h' three_quart ** tasks_res_own q three_quart
   )
   //** pure (t == h._1 /\ h == L.hd l /\ q == L.tl l)
 //ensures tasks_res_own (h::q) f
-ensures tasks_res_own (close_task_bis u#1 #task_elem t pos l) three_quart
+ensures tasks_res_own (close_task_bis u#1 #task t pos l) three_quart
 {
   rewrite (task_res_own h' three_quart ** tasks_res_own q three_quart) as (tasks_res_own (h'::q) three_quart);
   rewrite (tasks_res_own (h'::q) three_quart)
-    as (tasks_res_own (close_task_bis u#1 #task_elem t pos l) three_quart);
+    as (tasks_res_own (close_task_bis u#1 #task t pos l) three_quart);
   ()
 }
 ```
@@ -1061,7 +727,7 @@ ensures tasks_res_own (close_task_bis u#1 #task_elem t pos l) three_quart
 ```pulse
 ghost
 fn put_back_permission
-  (t: task_elem)
+  (t: task)
   (pos: nat)
   (l: (l:mono_list_task_plus{task_in_queue t pos l /\ L.length l >= 1}))
   (x: t._1)
@@ -1101,7 +767,7 @@ ensures tasks_res_own (close_task_bis t pos l) three_quart ** pure (
     rewrite (pts_to (h._1._2) #three_quart (Some x)) as (pts_to h'._1._2 #three_quart (Some x));
     fold_task_done h' three_quart;
     fold_tasks_res_own_bis h h' q pos t l;
-    assert (tasks_res_own (close_task_bis u#1 #task_elem t pos l) three_quart);
+    assert (tasks_res_own (close_task_bis u#1 #task t pos l) three_quart);
     ()
 
   }
@@ -1130,7 +796,7 @@ let prove_task_ongoing = prove_task_ongoing'
 ghost
 fn prove_ongoing_non_neg'
   (r:gmref)
-  (q: list task_elem) (c: int)
+  (q: list task) (c: int)
 requires small_inv r q c
 ensures small_inv r q c ** pure (c >= 0)
 {
@@ -1176,10 +842,10 @@ assume val drop (p: vprop): stt_ghost unit emp_inames p (fun () -> emp)
 ```pulse
 ghost
 fn conclude_task_ghost'
-(#t: task_elem)
+(#t: task)
 (#pos: nat)
 (r: gmref)
-(q: list task_elem) (c: int)
+(q: list task) (c: int)
 (x: t._1)
 (w: certificate r t pos)
   requires small_inv r q c ** pts_to t._2 #three_quart (Some x)
@@ -1192,16 +858,16 @@ fn conclude_task_ghost'
   with l. assert (M.pts_to r full_perm l);
   assert (tasks_res_own l three_quart);
   assert (pure (count_ongoing l = c /\ get_actual_queue l == q));
-  let proof = recall_full #task_elem #t #pos r l w;
+  let proof = recall_full #task #t #pos r l w;
   let p = close_task_bis t pos l;
-  let order_is_preserved = close_task_bis_preserves_order #task_elem t pos l;
-  write_ghost_queue #task_elem #l r p;
+  let order_is_preserved = close_task_bis_preserves_order #task t pos l;
+  write_ghost_queue #task #l r p;
   assert (M.pts_to r full_perm p);
 
   put_back_permission t pos l x;
   assert (tasks_res_own (close_task_bis t pos l) three_quart);
 
-  rewrite (tasks_res_own (close_task_bis u#1 #task_elem t pos (reveal u#1 #(mono_list u#1 task_elem) l)) three_quart)
+  rewrite (tasks_res_own (close_task_bis u#1 #task t pos (reveal u#1 #(mono_list u#1 task) l)) three_quart)
     as (tasks_res_own p three_quart);
 
   assert (M.pts_to r full_perm p);
@@ -1241,19 +907,19 @@ fn conclude_task_ghost'
 
 let conclude_task_ghost = conclude_task_ghost'
 
-let recall_certificate (#t: task_elem) (#pos: nat)
-           (r:ghost_mono_ref task_elem)
-           (v: mono_list task_elem)
+let recall_certificate (#t: task) (#pos: nat)
+           (r:ghost_mono_ref)
+           (v: mono_list task)
            (w:certificate r t pos)
 = recall_full r v w
 
 
-let pts_to_Some_fract (t:task_elem) (f: perm): vprop
+let pts_to_Some_fract (t:task) (f: perm): vprop
 = (exists_ (fun v -> pts_to t._2 #f v ** pure (Some? v)))
 
 // assuming recursion
 assume val get_Some_finished_aux_rec
-  (t: task_elem) (pos: nat)
+  (t: task) (pos: nat)
   (l: mono_list_task_plus)
   (f: perm)
 : stt_ghost unit emp_inames
@@ -1263,7 +929,7 @@ assume val get_Some_finished_aux_rec
 ```pulse
 ghost
 fn get_Some_finished_aux
-  (t: task_elem) (pos: nat)
+  (t: task) (pos: nat)
   (l: mono_list_task_plus)
   (f: perm)
 requires tasks_res_own l f ** pure (task_in_queue t pos l)
@@ -1289,7 +955,7 @@ ensures tasks_res_own l (half_perm f) ** pts_to_Some_fract t (half_perm f)
     //rewrite (pts_to_Some h (half_perm f)) as (pts_to_Some_fract t (half_perm f));
     //fold (pts_to_Some h (half_perm f));
     (*
-fn fold_task_done (h:(task_elem & task_status)) (f: perm)
+fn fold_task_done (h:(task & task_status)) (f: perm)
   requires pts_to h._1._2 #f (Some x) ** pure (h._2 = Done)
   ensures task_res_own h f
 {
@@ -1333,9 +999,9 @@ fn fold_task_done (h:(task_elem & task_status)) (f: perm)
 }
 ```
 
-let recall_certificate_fract (#t: task_elem) (#pos: nat)
-           (r:ghost_mono_ref task_elem)
-           (v: mono_list task_elem)
+let recall_certificate_fract (#t: task) (#pos: nat)
+           (r:ghost_mono_ref)
+           (v: mono_list task)
            (w:certificate r t pos)
            (f: perm):
  stt_ghost unit emp_inames
@@ -1347,7 +1013,7 @@ let recall_certificate_fract (#t: task_elem) (#pos: nat)
 
 ```pulse
 ghost fn
-proof_promise' (#t: task_elem) (#pos: nat)
+proof_promise' (#t: task) (#pos: nat)
   (r: gmref)
   (w:certificate r t pos)
 requires deadline r
@@ -1367,3 +1033,5 @@ ensures deadline r ** (exists_ (fun f -> (exists_ (fun v ->
 ```
 
 let proof_promise = proof_promise'
+
+*)
